src/Pact/CapabilityType.v
@@ -1,0 +1,81 @@
+Require Export
+  Lib
+  Value
+  RWSE.
+
+(* Set Universe Polymorphism. *)
+
+From Equations Require Import Equations.
+Set Equations With UIP.
+
+Generalizable All Variables.
+
+(*************************************************************************
+ * Capability values
+ *)
+
+Record CapSig : Set := {
+  paramTy : ValueTy;
+  valueTy : ValueTy;
+}.
+
+Derive NoConfusion NoConfusionHom Subterm EqDec for CapSig.
+
+Inductive Cap (s : CapSig) : Type :=
+  | Token (name : string) :
+    reflectTy (paramTy s) → reflectTy (valueTy s) → Cap s.
+
+Derive NoConfusion NoConfusionHom Subterm for Cap.
+
+#[export]
+Program Instance Cap_EqDec {s} : EqDec (Cap s).
+Next Obligation.
+  destruct x, y.
+  destruct (string_EqDec name name0); subst;
+  [|right; intro; congruence].
+  destruct (reflectTy_EqDec r r1); subst.
+  - destruct (reflectTy_EqDec r0 r2); subst.
+    + now left.
+    + right; intro; congruence.
+  - right; intro; congruence.
+Defined.
+
+Arguments Token {s} name arg val.
+
+Definition nameOf `(c : Cap s) : string :=
+  match c with Token n _ _ => n end.
+
+Definition paramOf `(c : Cap s) : reflectTy (paramTy s) :=
+  match c with Token _ p _ => p end.
+
+Definition valueOf `(c : Cap s) : reflectTy (valueTy s) :=
+  match c with Token _ _ v => v end.
+
+Inductive ACap : Type :=
+  | AToken (s : CapSig) : Cap s → ACap.
+
+Derive NoConfusion NoConfusionHom Subterm for ACap.
+
+#[export]
+Program Instance ACap_EqDec : EqDec ACap.
+Next Obligation.
+  destruct x, y.
+  destruct (CapSig_EqDec s s0); subst; [|right; congruence].
+  apply dec_eq_f1.
+  - apply Cap_EqDec.
+  - intros.
+    now inv H.
+Defined.
+
+Definition ACap_ext (ac : ACap) : { s : CapSig & Cap s } :=
+  match ac with AToken s c => existT _ s c end.
+
+Inductive CapError : Set :=
+  | CapErr_CapabilityNotAvailable
+  | CapErr_NoResourceAvailable
+  | CapErr_CannotInstallInDefcap
+  | CapErr_CannotWithInDefcap
+  | CapErr_CannotComposeOutsideDefcap
+  | CapErr_CannotWithOutsideDefcapModule.
+
+Derive NoConfusion NoConfusionHom Subterm EqDec for CapError.
